**16/11/2023**
___
$f(x)=x^n$ *->* $f'(x)=n \times x^{n-1}$
$f(x)=x^2$ *->* $f'(x)=2x$
$f(x)=x^{11}$ *->* $f'(x)=11y^{10}$
$f(x)=x^{-4}$ *->* $f'(x)=-4x^{-5}$
	$= \frac{1}{x^4} =- \frac{4}{x^5}$
___
**Faktorregel**: *$f(x)=a \times g(x)$ -> $f'(x)=a \times g'(x)$*

$f(x)=3 \times x^4$ *->* $f'(x)=3 \times 4x^3=12x^3$
$f(x)=7 \times x^5$ *->* $f'(x)=7 \times 5 \times x^4=35x^4$
$f(x)=-3 \times x^6$ *->* $f'(x)-3 \times 6 \times x^5=-18x^5$
$f(x)=-4x^{-3}$ *->* $f'(x)=-4 \times (-3) \times x^{-4}= \frac{12}{x^9}$
___
**Summenregel**: *$f(x)=g(x)+h(x)$ -> $f'(x)=g'(x)+h'(x)$*

$f(x)=x+x^2$ *->* $f'(x)=1+2x$
$f(x)=x^3+x^2$ *->* $f'(X)=3 \times x^2+2x$
$f(x)=x^6-3 \times x^2$ *->* $f'(x)=6x^5-6x$
$f(x)=x^{-2}+3x{-4}$ *->* $f'(x)=-2x^{-3}+3 \times (-4)x^{-5}=- \frac{2}{x^3} - \frac{12}{x^5}$
___
$f(x)=3x^4-3x^2+7$
*Bestimmen Sie die Steigung des Funktionsgraphen zu $f$ an der Stelle $x_1=2$ bzw. $x_0=-1$.*

$f'(x)=12x^3-6x$ | ==7 fÃ¤llt weg, da es sonst eine Gerade ist==
$f'(2)=84$ */* $f'(-1)=-6$
___
$f(x)=x^4-x^3+2x$ *;* $x_0=1$
	$f'(x)=4x^3-3x^2+2$
	$f'(-1)=3$

$f(x)=3x^3+2x^2-4$ *;* $x_0=-2$
	$f'(x)=9x^2+4x$
	$f'(-2)=28$

$f(x)=x^5+2x^2-3$ *;* $x_0=0$
	$f'(x)=5x^4+2 \times 2x$
	$f'(0)=0$
___
$f(x)=sin(x)$ *->* $f'(x)=cos(x)$
$f(x)=cos(x)$ *->* $f'(x)=-sin(x)$
$f(x)=-sin(x)$ *->* $f'(x)=-cos(x)$
$f'(x)=-cos(x)$ *->* $f'(x)=-(-sin(x))=sin(x)$

$f(x)=e^x$ *->* $f'(x)=e^x$ | ==e: Eulersche Zahl; $\approx 2,71 ...$==

$f(x)=ln(x)$ *->* $f'(x)= \frac{1}{x}$ | ==x>0==
___
**Produktregel**: $f(x)=g(x) \times h(x)$ *->* $f'(x)=g'(x) \times h(x)+g(x) \times h'(x)$

*Bsp.*: $f(x)=x^3 \times sin(x)$ *->* $g(x)=x^3$ *->* $g'(x)=3x^2$
					  $h(x)=sin(x)$ *->* $h'(x)=cos(x)$
*->* $f'(x)=3x^2 \times sin(x)+x^3 \times cos(x)$
	$=x^2(3sin(x)+x \times cos(x))$
___
$f(x)=x^2 \times e^x$ *->* $f'(x)=2x \times e^x+x^2 \times e^x=x \times e^x(2+x)$
